bodies

toy.dfy
@@ -11,73 +11,99 @@ class Global{
   predicate init()
   reads this;
   reads las, pas, l2p_ram, l2p_flash;
+  requires inv()
   {
-      //   N_LAS == 4000000
-      //&& N_PAS == 6000000
-      //&& N_DIFF == 4000000
-       0 <= p < N_DIFF
-      && las.Length == N_DIFF
-      && pas.Length == N_DIFF
-      && l2p_flash.Length == N_LAS
-      && l2p_ram.Length == N_LAS
-      && forall k: int :: 0 <= k < N_DIFF ==> las[k] == 0
-      && forall k: int :: 0 <= k < N_DIFF ==> pas[k] == 0
-      && forall k: int :: 0 <= k < N_LAS ==> l2p_ram[k] == 0
-      && forall k: int :: 0 <= k < N_LAS ==> l2p_flash[k] == 0
+    //   N_LAS == 4000000
+    //&& N_PAS == 6000000
+    //&& N_DIFF == 4000000
+       forall k: int :: 0 <= k < N_DIFF ==> las[k] == 0
+    && forall k: int :: 0 <= k < N_DIFF ==> pas[k] == 0
+    && forall k: int :: 0 <= k < N_LAS ==> l2p_ram[k] == 0
+    && forall k: int :: 0 <= k < N_LAS ==> l2p_flash[k] == 0
   }
   predicate inv()
   reads this;
   {
-    p < las.Length
+       0 <= p < N_DIFF
+    && las.Length == N_DIFF
+    && pas.Length == N_DIFF
+    && l2p_flash.Length == N_LAS
+    && l2p_ram.Length == N_LAS
   }
 }
 
-//method write (global0: Global, la: int, pa: int) returns (global1: Global)
-//  modifies global0.l2p_ram;
-//  modifies global0.las;
-//  modifies global0.pas;
-//  modifies global0;
-//  requires global0.init();
-//  ensures 0 <= global1.p < global1.N_DIFF
-//  ensures la >= global0.N_LAS || pa >= global0.N_PAS ==> global0 == global1;
-//  ensures global1.l2p_flash.Length == global1.N_LAS == global1.l2p_ram.Length
-//  ensures la < global0.N_LAS && pa < global0.N_PAS ==>
-//    global1.p == global1.N_DIFF - 1 ==> forall k: int :: 0 <= k < global1.N_LAS ==> global1.l2p_flash[k] == global1.l2p_ram[k]
-//{
-//    global1 := global0;
-//    assert 0 <= global1.p < global1.N_DIFF;
-//    assert global1.l2p_flash.Length == global1.N_LAS;
-//    assert global1.l2p_ram.Length == global1.N_LAS;
-//    if (la >= global1.N_LAS || pa >= global1.N_PAS)
-//      { return global1; }
-//    assert la < global0.N_LAS && pa < global1.N_PAS;
-//    global1.l2p_ram[global1.p] := pa;
-//    global1.las[global1.p] := la;
-//    global1.pas[global1.p] := pa;
-//    global1.p := global1.p + 1;
-//    if (global1.p == global1.N_DIFF)
-//      {
-//          global1.p := 0;
-//          var i := 0;
-//          while (i < global1.N_LAS)
-//            invariant forall k: int :: 0 <= k < global1.N_LAS ==> global1.l2p_flash[k] == global1.l2p_ram[k]
-//          {
-//              global1.l2p_flash[i] :=  global1.l2p_ram[i];
-//              i := i + 1;
-//          }
-//      }
-//    //assert global0.p < global0.N_DIFF ==> global1.p == global0.p + 1;
-//    assert global0.p == global0.N_DIFF ==> global1.p < global0.p + 1;
-//    return global1;
-//}
+method write (global0: Global, la: int, pa: int) returns (global1: Global)
+  modifies global0.l2p_ram;
+  modifies global0.l2p_flash;
+  modifies global0.las;
+  modifies global0.pas;
+  modifies global0;
+  requires global0.inv();
+  requires 0 <= la && 0 <= pa;
+  //ensures 0 <= global1.p < global1.N_DIFF
+  //ensures la >= global0.N_LAS || pa >= global0.N_PAS ==> global0 == global1;
+  //ensures global1.l2p_flash.Length == global1.N_LAS == global1.l2p_ram.Length
+  //ensures la < global0.N_LAS && pa < global0.N_PAS ==>
+  //  global1.p == global1.N_DIFF - 1 ==> forall k: int :: 0 <= k < global1.N_LAS ==> global1.l2p_flash[k] == global1.l2p_ram[k]
+{
+    global1 := global0;
+    assert 0 <= global1.p < global1.N_DIFF;
+    assert global1.l2p_flash.Length == global1.N_LAS;
+    assert global1.l2p_ram.Length == global1.N_LAS;
+    if (la >= global1.N_LAS || la < 0 || pa >= global1.N_PAS || pa < 0)
+      { return global1; }
+    assert la < global1.N_LAS && pa < global1.N_PAS;
+    global1.l2p_ram[la] := pa;
+    global1.las[global1.p] := la;
+    global1.pas[global1.p] := pa;
+    global1.p := global1.p + 1;
+    if (global1.p == global1.N_DIFF)
+      {
+          global1.p := 0;
+          var i := 0;
+          while (i < global1.N_LAS)
+            invariant 0 <= i <= global1.N_LAS
+            modifies global1.l2p_flash;
+            //invariant forall k: int :: 0 <= k < global1.N_LAS ==> global1.l2p_flash[k] == global1.l2p_ram[k]
+          {
+              assert i < global1.N_LAS;
+              global1.l2p_flash[i] :=  global1.l2p_ram[i];
+              i := i + 1;
+          }
+      }
+    //assert global0.p < global0.N_DIFF ==> global1.p == global0.p + 1;
+    assert global0.p == global0.N_DIFF ==> global1.p < global0.p + 1;
+    return global1;
+}
+
+lemma AllRI(global: Global)
+  requires global.inv()
+{
+  var i := 0;
+  var bnd := i + 1;
+  RI(global, i);
+  while(bnd < global.p)
+    invariant exists lbnd | i <= lbnd <= global.p ::
+                            global.las[i] == global.las[lbnd]
+                         && notin(lbnd, global.p, global.las[i], global.las);
+    invariant i <= bnd;
+  {
+    i := i + 1;
+    RI(global, i);
+    bnd := bnd + 1;
+  }
+  assert exists lbnd | i <= lbnd <= global.p ::
+                global.las[i] == global.las[lbnd]
+             && notin(lbnd, global.p, global.las[i], global.las);
+}
 
 lemma RI(global: Global, i: int)
-  requires global.init()
-  //requires global.inv()
+  //requires global.init()
+  requires global.inv()
   requires 0 <= i <= global.p
-  ensures forall j | 0 <= j <= global.p ::
-            exists lbnd | j <= lbnd <= global.p ::
-                     global.las[j] == global.las[lbnd] && notin(lbnd, global.p, global.las[j], global.las);
+  ensures exists lbnd | i <= lbnd <= global.p ::
+                      global.las[i] == global.las[lbnd]
+                   && notin(lbnd, global.p, global.las[i], global.las);
 {
   var lbnd := i;
   var rbnd := i;
